core/Prog.v
@@ -1,4 +1,4 @@
-Require Import Monads ProofMonads List ZArith Program.
+(* Require Import Monads ProofMonads List ZArith Program.
 
 Open Scope monad_scope.
 
@@ -166,3 +166,4 @@ Compute runState (
   ) init_Z1.
 
 End Test.
+ *)
